src/Parsers/Refinement/SharpenedABStar.v
@@ -44,59 +44,7 @@ Defined.
 
 Definition ab_star_parser_ocaml (str : Ocaml.Ocaml.string) : bool.
 Proof.
-(*Declare Reduction parser_red0' := cbv beta iota zeta delta [list_to_grammar item_ascii_cons item_of_char list_to_productions BooleanRecognizerOptimized.str_carrier_default projT1 projT2 proj1_sig proj2_sig].
-Declare Reduction parser_red4' := cbv beta iota zeta delta [ParserInterface.has_parse ParserFromParserADT.parser projT1 projT2 ComputationalADT.pcMethods ComputationalADT.pcConstructors ilist.ith VectorFacts.Vector_caseS' Vector.caseS ilist.ilist_hd ilist.ilist_tl ilist.prim_fst ilist.prim_snd BooleanRecognizerOptimized.of_string BooleanRecognizerOptimized.to_string StringLike.String StringLike.length StringLike.take StringLike.drop StringLike.get StringLike.is_char StringLike.bool_eq StringLike.beq string_stringlike RDPList.rdp_list_to_production Carriers.default_to_production].
-Global Arguments BooleanRecognizerOptimized.inner_nth' {_} _ !_ _ / .
-  Time let splitter := ComputationalSplitter in
-  let do_simpl_list_map := true in
-    idtac;
-  let str := match goal with
-               | [ str : String.string |- _ ] => constr:str
-               | [ str : Ocaml.Ocaml.string |- _ ] => constr:str
-             end in
-  let b0 := constr:(fun pf => ParserInterface.has_parse (ParserFromParserADT.parser pf splitter) str) in
-  let T := match type of b0 with ?T -> _ => constr:T end in
-  let quicker_opaque_eq_refl := constr:(_ : eq_refl_vm_cast T) in
-  let b := constr:(b0 quicker_opaque_eq_refl) in
-  let b' := let term := b in
-  let term := match term with
-                | context[ParserFromParserADT.parser _ ?splitter]
-                  => let splitter' := head splitter in
-                     (eval unfold splitter' in term)
-                | _ => constr:term
-              end in
-  let term := (eval parser_red0 in term) in
-  let term := (eval parser_red1 in term) in
-  let term := (eval parser_red2 in term) in
-  let term := (eval parser_red3 in term) in
-  let term := (eval parser_red4 in term) in
-  let term := (eval cbv beta iota zeta delta [BooleanRecognizerOptimized.rdp_list_to_production_opt item_rect] in term) in
-  let term := (eval parser_red5 in term) in
-  let term := (eval parser_red6 in term) in
-  let term := (eval parser_red7 in term) in
-  let term := (eval parser_red8 in term) in
-  let term := (eval parser_red9 in term) in
-  let term := (eval parser_red10 in term) in
-  let term := (eval parser_red11 in term) in
-  let term := (eval parser_red12 in term) in
-  let term := (eval parser_red13 in term) in
-  let term := (eval parser_red14 in term) in
-  let term := (eval simpl @BooleanRecognizerOptimized.inner_nth' in term) in
-  let term := (eval simpl @List.fold_left in term) in(*
-  let term := (match do_simpl_list_map with
-                 | true => eval simpl List.map in term
-                 | _ => term
-               end) in
-  let term := (eval parser_red16 in term) in*)
-  constr:term in
-  (*let b' := (eval cbv beta iota zeta delta [RDPList.rdp_list_to_production Carriers.default_to_production] in b') in
-  let b' := parser_red_gen b' do_simpl_list_map in*)
-  pose b'.
-  .
-  parser_red0 in *.
-  simpl @RDPList.rdp_list_to_production
-  Time make_parser ComputationalSplitter. (* 0.6 s *)*)
-  Time make_parser ComputationalSplitter. (* 0.6 s *)
+  Time make_parser (@ComputationalSplitter Ocaml.string_stringlike _ _). (* 0.82 s *)
 Defined.
 
 Print ab_star_parser_ocaml.
